allow bindings to throw exceptions for ELet (not ILet)

coq-osiris/theories/program_logic/pure/binding_rules.v
@@ -6,16 +6,25 @@ From osiris.program_logic.pure Require Import wp judgements pattern_rules.
 
 (* A judgement for the evaluation of let bindings. *)
 
-Definition bindings η bs (φ : env -> Prop) :=
-  pure_wp (eval_bindings η bs) φ (λ _, False).
+Definition bindings η bs (φ : env -> Prop) (ψ : exn -> Prop) :=
+  pure_wp (eval_bindings η bs) φ ψ.
+
+Lemma pure_wp_irrefutably_extend η δ p v φ ψ :
+  pure_wp (extend η δ p v) φ ⊥ →
+  pure_wp (irrefutably_extend η δ p v) φ ψ.
+Proof.
+  intros H.
+  apply pure_wp_try, (pure_wp_mono _ H);
+    firstorder eauto with pure.
+Qed.
 
 (* -------------------------------------------------------------------------- *)
 
 (* Syntax-directed reasoning rules for the auxiliary judgement [bindings]. *)
 
 Lemma bindings_cons_unary `{Encode A} η p e bs φ :
-  pure (eval η e) (λ a : A, bindings η bs (λ η', pattern η η' p #a φ False)) ⊥ ->
-  bindings η (Binding p e :: bs) φ.
+  pure (eval η e) (λ a : A, bindings η bs (λ η', pattern η η' p #a φ False) ⊥) ⊥ ->
+  bindings η (Binding p e :: bs) φ ⊥.
 Proof.
   unfold bindings. simpl. intros He.
   simpl_eval_bindings.
@@ -26,32 +35,35 @@ Proof.
   intros. by apply pure_wp_ret. intros _ [].
 Qed.
 
-Lemma bindings_cons `{Encode A} η p e bs φ φ' (ψ : A -> Prop) :
-  pure (eval η e) ψ ⊥ ->
-  bindings η bs φ' ->
-  (∀ (x : A) (η' : env), ψ x -> φ' η' -> pattern η η' p #x φ False) ->
-  bindings η (Binding p e :: bs) φ.
+Lemma bindings_cons `{Encode A} η p e bs (φ1 : A -> Prop) φ2 φ ψ :
+  pure (eval η e) φ1 ψ ->
+  bindings η bs φ2 ψ ->
+  (∀ (a : A) (η' : env), φ1 a -> φ2 η' -> pattern η η' p #a φ False) ->
+  bindings η (Binding p e :: bs) φ ψ.
 Proof.
   intros He Hbs Hp.
-  eapply bindings_cons_unary.
-  apply (pure_wp_mono_ret _ He). intros v (a & -> & Ha). exists a. split; auto.
-  apply (pure_wp_mono_ret _ Hbs). eauto.
+  unfold bindings.
+  simpl_eval_bindings.
+  eapply pure_wp_Par_conseq; eauto.
+  - intros _ η' (a & -> & Ha) Hη'.
+    eapply pure_wp_bind, pure_wp_ret, pure_wp_widen, pure_wp_irrefutably_extend. apply Hp; eauto.
+  - intros. eapply pure_wp_bind, pure_wp_throw. tauto.
 Qed.
 
-Lemma bindings_nil `{Encode A} η (φ : env -> Prop) :
+Lemma bindings_nil `{Encode A} η (φ : env -> Prop) ψ :
   φ [] ->
-  bindings η [] φ.
+  bindings η [] φ ψ.
 Proof.
   unfold bindings. simpl_eval_bindings. apply pure_wp_ret.
 Qed.
 
-Lemma bindings_var `{Encode A} η v e bs φ' (ψ : A -> Prop) :
-  pure (eval η e) ψ ⊥ ->
-  bindings η bs φ' ->
+Lemma bindings_var `{Encode A} η v e bs (φ : A -> Prop) φ' ψ :
+  pure (eval η e) φ ψ ->
+  bindings η bs φ' ψ ->
   bindings η
     (Binding (PVar v) e :: bs)
     (λ η,
-      ∃ a η', ψ a /\ φ' η' /\ η = (v, #a) :: η').
+      ∃ a η', φ a /\ φ' η' /\ η = (v, #a) :: η') ψ.
 Proof.
   intros.
   eapply bindings_cons; eauto.
@@ -60,13 +72,13 @@ Proof.
 Qed.
 
 Lemma bindings_pair `{Encode A, Encode B} η p1 p2 e bs φ φ'
-  (ψ1 : A -> Prop) (ψ2 : B -> Prop) :
-  pure (eval η e) (λ '(a, b), ψ1 a /\ ψ2 b) ⊥ ->
-  bindings η bs φ' ->
-  (∀ a b η', ψ1 a -> ψ2 b -> φ' η' -> pattern η η' (PPair p1 p2) #(a, b) φ False) ->
-  bindings η (Binding (PPair p1 p2) e :: bs) φ.
+  (φ1 : A -> Prop) (φ2 : B -> Prop) ψ :
+  pure (eval η e) (λ '(a, b), φ1 a /\ φ2 b) ψ ->
+  bindings η bs φ' ψ ->
+  (∀ a b η', φ1 a -> φ2 b -> φ' η' -> pattern η η' (PPair p1 p2) #(a, b) φ False) ->
+  bindings η (Binding (PPair p1 p2) e :: bs) φ ψ.
 Proof.
-    intros Hpure Hbs Hpat.
+  intros Hpure Hbs Hpat.
   eapply bindings_cons; eauto.
   intros [a b] η' [Hψ1 Hψ2] Hη'.
   auto.
